ulib/FStar.Tactics.Effect.fsti
@@ -22,103 +22,113 @@ open FStar.Tactics.Result
 (* This module is extracted, don't add any `assume val`s or extraction
  * will break. (`synth_by_tactic` is fine) *)
 
-private
-let __tac (a:Type) = proofstate -> M (__result a)
+val ugh : unit
 
-(* monadic return *)
-private
-let __ret (a:Type) (x:a) : __tac a = fun (s:proofstate) -> Success x s
-
-(* monadic bind *)
-private
-let __bind (a:Type) (b:Type) (r1 r2:range) (t1:__tac a) (t2:a -> __tac b) : __tac b =
-    fun ps ->
-        let ps = set_proofstate_range ps (FStar.Range.prims_to_fstar_range r1) in
-        let ps = incr_depth ps in
-        let r = t1 ps in
-        match r with
-        | Success a ps' ->
-            let ps' = set_proofstate_range ps' (FStar.Range.prims_to_fstar_range r2) in
-            // Force evaluation of __tracepoint q even on the interpreter
-            begin match tracepoint ps' with
-            | true -> t2 a (decr_depth ps')
-            end
-        | Failed e ps' -> Failed e ps'
-
-(* Actions *)
-private
-let __get () : __tac proofstate = fun s0 -> Success s0 s0
-
-private
-let __raise (a:Type0) (e:exn) : __tac a = fun (ps:proofstate) -> Failed #a e ps
-
-private
-let __tac_wp a = proofstate -> (__result a -> Tot Type0) -> Tot Type0
-
-(* The DMFF-generated `bind_wp` doesn't the contain the "don't
- * duplicate the post-condition" optimization, which causes VCs (for
- * well-formedness of tactics) to blow up.
- *
- * Plus, we don't need to model the ranges and depths: they make no
- * difference since the proofstate type is abstract and the SMT never
- * sees a concrete one.
- *
- * So, override `bind_wp` for the effect with an efficient one.
- *)
-private
-unfold let g_bind (a:Type) (b:Type) (wp:__tac_wp a) (f:a -> __tac_wp b) = fun ps post ->
-    wp ps (fun m' -> match m' with
-                     | Success a q -> f a q post
-                     | Failed e q -> post (Failed e q))
-
-private
-unfold let g_compact (a:Type) (wp:__tac_wp a) : __tac_wp a =
-    fun ps post -> forall k. (forall (r:__result a).{:pattern (guard_free (k r))} post r ==> k r) ==> wp ps k
-
-private
-unfold let __TAC_eff_override_bind_wp (r:range) (a:Type) (b:Type) (wp:__tac_wp a) (f:a -> __tac_wp b) =
-    g_compact b (g_bind a b wp f)
-
-[@@ dm4f_bind_range ]
-new_effect {
-  TAC : a:Type -> Effect
-  with repr     = __tac
-     ; bind     = __bind
-     ; return   = __ret
-     ; __raise  = __raise
-     ; __get    = __get
-}
-
-(* Hoare variant *)
-effect TacH (a:Type) (pre : proofstate -> Tot Type0) (post : proofstate -> __result a -> Tot Type0) =
-    TAC a (fun ps post' -> pre ps /\ (forall r. post ps r ==> post' r))
-
-(* "Total" variant *)
-effect Tac (a:Type) = TacH a (requires (fun _ -> True)) (ensures (fun _ _ -> True))
-
-(* Metaprograms that succeed *)
-effect TacS (a:Type) = TacH a (requires (fun _ -> True)) (ensures (fun _ps r -> Success? r))
-
-(* A variant that doesn't prove totality (nor type safety!) *)
-effect TacF (a:Type) = TacH a (requires (fun _ -> False)) (ensures (fun _ _ -> True))
+type wp_t0 (a:Type) = proofstate -> (__result a -> Type0) -> Type0
 
 unfold
-let lift_div_tac (a:Type) (wp:pure_wp a) : __tac_wp a =
-    fun ps p -> wp (fun x -> p (Success x ps))
+let monotonic (#a:Type) (wp:wp_t0 a) =
+  forall ps p q. (forall x. p x ==> q x) ==> (wp ps p ==> wp ps q)
 
-sub_effect DIV ~> TAC = lift_div_tac
+type wp_t (a:Type) = wp:wp_t0 a{monotonic wp}
 
-let get = TAC?.__get
-let raise (#a:Type) (e:exn) = TAC?.__raise a e
+type repr (a:Type) (wp:wp_t a) = ps:proofstate -> PURE (__result a) (wp ps)
+
+unfold
+let return_wp (#a:Type) (x:a) : wp_t a = fun ps p -> p (Success x ps)
+let return (a:Type) (x:a) : repr a (return_wp x) = fun ps -> Success x ps
+
+unfold
+let g_bind (a:Type) (b:Type) (wp:wp_t a) (f:a -> wp_t b) : wp_t b =
+  fun ps post ->
+  wp ps (fun m' -> match m' with
+                | Success a q -> f a q post
+                | Failed e q -> post (Failed e q))
+unfold
+let g_compact (a:Type) (wp:wp_t a) : wp_t a =
+    fun ps post -> forall k. (forall (r:__result a).{:pattern (guard_free (k r))} post r ==> k r) ==> wp ps k
+
+#push-options "--admit_smt_queries true"
+let bind (a b:Type)
+  //(r1 r2:range)
+  (wp1:wp_t a) (wp2:a -> wp_t b)
+  (t1:repr a wp1) (t2:(x:a -> repr b (wp2 x)))
+  : repr b (g_compact b (g_bind a b wp1 wp2)) =
+  fun ps ->
+  //let ps = set_proofstate_range ps (FStar.Range.prims_to_fstar_range r1) in
+  let ps = incr_depth ps in
+  let r = t1 ps in
+  match r with
+  | Success a ps' ->
+    //let ps' = set_proofstate_range ps' (FStar.Range.prims_to_fstar_range r2) in
+    // Force evaluation of __tracepoint q even on the interpreter
+    begin match tracepoint ps' with
+          | true -> t2 a (decr_depth ps')
+    end
+  | Failed e ps' -> Failed e ps'
+#pop-options
+
+let subcomp (a:Type) (wp1 wp2:wp_t a)
+  (f:repr a wp1)
+  : Pure (repr a wp2)
+      (requires forall ps p. wp2 ps p ==> wp1 ps p)
+      (ensures fun _ -> True)
+  = f
+
+unfold
+let if_then_else_wp (#a:Type) (wp1 wp2:wp_t a) (b:bool) : wp_t a =
+  fun ps p -> (b ==> wp1 ps p) /\
+           ((~ b) ==> wp2 ps p)
+
+let if_then_else (a:Type) (wp1 wp2:wp_t a)
+  (f:repr a wp1) (g:repr a wp2)
+  (b:bool)
+  : Type =
+  repr a (if_then_else_wp wp1 wp2 b)
+
+reifiable
+reflectable
+effect {
+  TAC (a:Type) (wp:wp_t a)
+  with {repr; return; bind; subcomp; if_then_else}
+}
+
+effect TacH (a:Type) (pre:proofstate -> Type0) (post:proofstate -> __result a -> Type0) =
+  TAC a (fun ps post' -> pre ps /\ (forall r. post ps r ==> post' r))
+
+effect Tac (a:Type) = TacH a (requires fun _ -> True) (ensures fun _ _ -> True)
+
+effect TacS (a:Type) = TacH a (requires fun _ -> True) (ensures fun _ r -> Success? r)
+
+effect TacF (a:Type) = TacH a (requires fun _ -> False) (ensures fun _ _ -> True)
+
+unfold
+let lift_pure_tac_wp (#a:Type) (wp:pure_wp a) : wp_t a =
+  FStar.Monotonic.Pure.wp_monotonic_pure ();
+  fun ps p -> wp (fun x -> p (Success x ps))
+
+let lift_pure_tac (a:Type) (wp:pure_wp a) (f:eqtype_as_type unit -> PURE a wp)
+  : repr a (lift_pure_tac_wp wp)
+  =  FStar.Monotonic.Pure.wp_monotonic_pure ();
+     fun ps -> Success (f ()) ps
+
+sub_effect PURE ~> TAC = lift_pure_tac
+
+let get () : TAC proofstate (fun ps p -> p (Success ps ps)) =
+  TAC?.reflect (fun ps -> Success ps ps)
+
+let raise (#a:Type) (e:exn) : TAC a (fun ps p -> p (Failed #a e ps)) =
+  TAC?.reflect (fun ps -> Failed #a e ps)
+
 
 val with_tactic (t : unit -> Tac unit) (p:Type u#a) : Type u#a
 
 (* This will run the tactic in order to (try to) produce a term of type
- * t. Note that the type looks dangerous from a logical perspective. It
- * should not lead to any inconsistency, however, as any time this term
- * appears during typechecking, it is forced to be fully applied and the
- * tactic is run. A failure of the tactic is a typechecking failure. It
- * can be thought as a language construct, and not a real function. *)
+//  * t. Note that the type looks dangerous from a logical perspective. It
+//  * should not lead to any inconsistency, however, as any time this term
+//  * appears during typechecking, it is forced to be fully applied and the
+//  * tactic is run. A failure of the tactic is a typechecking failure. It
+//  * can be thought as a language construct, and not a real function. *)
 val synth_by_tactic : (#t:Type) -> (unit -> Tac unit) -> Tot t
 
 val assert_by_tactic (p:Type) (t:unit -> Tac unit)
@@ -127,38 +137,38 @@ val assert_by_tactic (p:Type) (t:unit -> Tac unit)
          (ensures (fun _ -> p))
 
 (* We don't peel off all `with_tactic`s in negative positions, so give
- * the SMT a way to reason about them *)
+//  * the SMT a way to reason about them *)
 val by_tactic_seman : tau:(unit -> Tac unit) -> phi:Type -> Lemma (with_tactic tau phi ==> phi)
                                                                   [SMTPat (with_tactic tau phi)]
 
 (* One can always bypass the well-formedness of metaprograms. It does
- * not matter as they are only run at typechecking time, and if they get
- * stuck, the compiler will simply raise an error. *)
+//  * not matter as they are only run at typechecking time, and if they get
+//  * stuck, the compiler will simply raise an error. *)
 let assume_safe (#a:Type) (tau:unit -> TacF a) : Tac a = admit (); tau ()
 
 private let tac a b = a -> Tac b
 private let tactic a = tac unit a
 
 (* A hook to preprocess a definition before it is typechecked and
- * elaborated. This attribute should be used for top-level lets. The
- * tactic [tau] will be called on a quoting of the definition of the let
- * (if many, once for each) and the result of the tactic will replace
- * the definition. There are no goals involved, nor any proof obligation
- * to be done by the tactic. *)
+//  * elaborated. This attribute should be used for top-level lets. The
+//  * tactic [tau] will be called on a quoting of the definition of the let
+//  * (if many, once for each) and the result of the tactic will replace
+//  * the definition. There are no goals involved, nor any proof obligation
+//  * to be done by the tactic. *)
 val preprocess_with (tau : term -> Tac term) : Tot unit
 
 (* A hook to postprocess a definition, after typechecking, and rewrite
- * it into a (provably equal) shape chosen by the user. This can be used
- * to implement custom transformations previous to extraction, such as
- * selective inlining. When ran added to a definition [let x = E], the
- * [tau] metaprogram is presented with a goal of the shape [E == ?u] for
- * a fresh uvar [?u]. The metaprogram should then both instantiate [?u]
- * and prove the equality. *)
+//  * it into a (provably equal) shape chosen by the user. This can be used
+//  * to implement custom transformations previous to extraction, such as
+//  * selective inlining. When ran added to a definition [let x = E], the
+//  * [tau] metaprogram is presented with a goal of the shape [E == ?u] for
+//  * a fresh uvar [?u]. The metaprogram should then both instantiate [?u]
+//  * and prove the equality. *)
 val postprocess_with (tau : unit -> Tac unit) : Tot unit
 
 (* Similar semantics to [postprocess_with], but the metaprogram only
- * runs before extraction, and hence typechecking and the logical
- * environment should not be affected at all. *)
+//  * runs before extraction, and hence typechecking and the logical
+//  * environment should not be affected at all. *)
 val postprocess_for_extraction_with (tau : unit -> Tac unit) : Tot unit
 
 #set-options "--no_tactics"
@@ -166,3 +176,170 @@ val postprocess_for_extraction_with (tau : unit -> Tac unit) : Tot unit
 val unfold_with_tactic (t:unit -> Tac unit) (p:Type)
   : Lemma (requires p)
           (ensures (with_tactic t p))
+
+// let bind (a:Type) (b:Type) (t1:__tac a) (t2:a -> __tac b) : __tac b =
+//     fun ps ->
+//         let ps = set_proofstate_range ps (FStar.Range.prims_to_fstar_range r1) in
+//         let ps = incr_depth ps in
+//         let r = t1 ps in
+//         match r with
+//         | Success a ps' ->
+//             let ps' = set_proofstate_range ps' (FStar.Range.prims_to_fstar_range r2) in
+//             // Force evaluation of __tracepoint q even on the interpreter
+//             begin match tracepoint ps' with
+//             | true -> t2 a (decr_depth ps')
+//             end
+//         | Failed e ps' -> Failed e ps'
+
+
+
+
+
+// private
+// let __tac (a:Type) = proofstate -> M (__result a)
+
+// (* monadic return *)
+// private
+// let __ret (a:Type) (x:a) : __tac a = fun (s:proofstate) -> Success x s
+
+// (* monadic bind *)
+// private
+// let __bind (a b:Type)
+//   //(r1 r2:range)
+//   (wp1:wp_t a) (wp2:a -> wp_t b)
+//   (t1:repr a wp1) (t2:(x:a -> repr b (wp2 x)))
+//   : repr b ( =
+//     fun ps ->
+//         let ps = set_proofstate_range ps (FStar.Range.prims_to_fstar_range r1) in
+//         let ps = incr_depth ps in
+//         let r = t1 ps in
+//         match r with
+//         | Success a ps' ->
+//             let ps' = set_proofstate_range ps' (FStar.Range.prims_to_fstar_range r2) in
+//             // Force evaluation of __tracepoint q even on the interpreter
+//             begin match tracepoint ps' with
+//             | true -> t2 a (decr_depth ps')
+//             end
+//         | Failed e ps' -> Failed e ps'
+
+// (* Actions *)
+// private
+// let __get () : __tac proofstate = fun s0 -> Success s0 s0
+
+// private
+// let __raise (a:Type0) (e:exn) : __tac a = fun (ps:proofstate) -> Failed #a e ps
+
+// private
+// let __tac_wp a = proofstate -> (__result a -> Tot Type0) -> Tot Type0
+
+// (* The DMFF-generated `bind_wp` doesn't the contain the "don't
+//  * duplicate the post-condition" optimization, which causes VCs (for
+//  * well-formedness of tactics) to blow up.
+//  *
+//  * Plus, we don't need to model the ranges and depths: they make no
+//  * difference since the proofstate type is abstract and the SMT never
+//  * sees a concrete one.
+//  *
+//  * So, override `bind_wp` for the effect with an efficient one.
+//  *)
+// private
+// unfold let g_bind (a:Type) (b:Type) (wp:__tac_wp a) (f:a -> __tac_wp b) = fun ps post ->
+//     wp ps (fun m' -> match m' with
+//                      | Success a q -> f a q post
+//                      | Failed e q -> post (Failed e q))
+
+// private
+// unfold let g_compact (a:Type) (wp:__tac_wp a) : __tac_wp a =
+//     fun ps post -> forall k. (forall (r:__result a).{:pattern (guard_free (k r))} post r ==> k r) ==> wp ps k
+
+// private
+// unfold let __TAC_eff_override_bind_wp (r:range) (a:Type) (b:Type) (wp:__tac_wp a) (f:a -> __tac_wp b) =
+//     g_compact b (g_bind a b wp f)
+
+// [@@ dm4f_bind_range ]
+// new_effect {
+//   TAC : a:Type -> Effect
+//   with repr     = __tac
+//      ; bind     = __bind
+//      ; return   = __ret
+//      ; __raise  = __raise
+//      ; __get    = __get
+// }
+
+// (* Hoare variant *)
+// effect TacH (a:Type) (pre : proofstate -> Tot Type0) (post : proofstate -> __result a -> Tot Type0) =
+//     TAC a (fun ps post' -> pre ps /\ (forall r. post ps r ==> post' r))
+
+// (* "Total" variant *)
+// effect Tac (a:Type) = TacH a (requires (fun _ -> True)) (ensures (fun _ _ -> True))
+
+// (* Metaprograms that succeed *)
+// effect TacS (a:Type) = TacH a (requires (fun _ -> True)) (ensures (fun _ps r -> Success? r))
+
+// (* A variant that doesn't prove totality (nor type safety!) *)
+// effect TacF (a:Type) = TacH a (requires (fun _ -> False)) (ensures (fun _ _ -> True))
+
+// unfold
+// let lift_div_tac (a:Type) (wp:pure_wp a) : __tac_wp a =
+//     fun ps p -> wp (fun x -> p (Success x ps))
+
+// sub_effect DIV ~> TAC = lift_div_tac
+
+// let get = TAC?.__get
+// let raise (#a:Type) (e:exn) = TAC?.__raise a e
+
+// val with_tactic (t : unit -> Tac unit) (p:Type u#a) : Type u#a
+
+// (* This will run the tactic in order to (try to) produce a term of type
+//  * t. Note that the type looks dangerous from a logical perspective. It
+//  * should not lead to any inconsistency, however, as any time this term
+//  * appears during typechecking, it is forced to be fully applied and the
+//  * tactic is run. A failure of the tactic is a typechecking failure. It
+//  * can be thought as a language construct, and not a real function. *)
+// val synth_by_tactic : (#t:Type) -> (unit -> Tac unit) -> Tot t
+
+// val assert_by_tactic (p:Type) (t:unit -> Tac unit)
+//   : Pure unit
+//          (requires (set_range_of (with_tactic t (squash p)) (range_of t)))
+//          (ensures (fun _ -> p))
+
+// (* We don't peel off all `with_tactic`s in negative positions, so give
+//  * the SMT a way to reason about them *)
+// val by_tactic_seman : tau:(unit -> Tac unit) -> phi:Type -> Lemma (with_tactic tau phi ==> phi)
+//                                                                   [SMTPat (with_tactic tau phi)]
+
+// (* One can always bypass the well-formedness of metaprograms. It does
+//  * not matter as they are only run at typechecking time, and if they get
+//  * stuck, the compiler will simply raise an error. *)
+// let assume_safe (#a:Type) (tau:unit -> TacF a) : Tac a = admit (); tau ()
+
+// private let tac a b = a -> Tac b
+// private let tactic a = tac unit a
+
+// (* A hook to preprocess a definition before it is typechecked and
+//  * elaborated. This attribute should be used for top-level lets. The
+//  * tactic [tau] will be called on a quoting of the definition of the let
+//  * (if many, once for each) and the result of the tactic will replace
+//  * the definition. There are no goals involved, nor any proof obligation
+//  * to be done by the tactic. *)
+// val preprocess_with (tau : term -> Tac term) : Tot unit
+
+// (* A hook to postprocess a definition, after typechecking, and rewrite
+//  * it into a (provably equal) shape chosen by the user. This can be used
+//  * to implement custom transformations previous to extraction, such as
+//  * selective inlining. When ran added to a definition [let x = E], the
+//  * [tau] metaprogram is presented with a goal of the shape [E == ?u] for
+//  * a fresh uvar [?u]. The metaprogram should then both instantiate [?u]
+//  * and prove the equality. *)
+// val postprocess_with (tau : unit -> Tac unit) : Tot unit
+
+// (* Similar semantics to [postprocess_with], but the metaprogram only
+//  * runs before extraction, and hence typechecking and the logical
+//  * environment should not be affected at all. *)
+// val postprocess_for_extraction_with (tau : unit -> Tac unit) : Tot unit
+
+// #set-options "--no_tactics"
+
+// val unfold_with_tactic (t:unit -> Tac unit) (p:Type)
+//   : Lemma (requires p)
+//           (ensures (with_tactic t p))
