ulib/FStar.Tactics.CanonMonoid.fst
@@ -21,7 +21,7 @@ open FStar.Tactics
 open FStar.Reflection
 
 (* Only dump when debugging is on *)
-let dump m = if debugging () then dump m
+let dump m : Tac _ = if debugging () then dump m
 
 (* "A Monoid Expression Simplifier" ported from
    http://adam.chlipala.net/cpdt/html/Cpdt.Reflection.html *)
